More on cycles

experiments/Cycles.thy
@@ -5,14 +5,13 @@ imports "../Llists_Processors"
 begin
 
 coinductive le_op where
-   "lprefix (buf1 @@- exit op1) (buf2 @@- exit op2) \<Longrightarrow>
-    (\<And> ev op1' op2' out1 out2. 
+   "lprefix (buf1 @@- exit op1) (buf2 @@- exit op2) \<Longrightarrow> prefix buf1 buf2 \<Longrightarrow>
+    (\<And> ev op1' op2' out1 out2.
       apply op1 ev = (op1', out1) \<Longrightarrow> apply op2 ev = (op2', out2) \<Longrightarrow> le_op op1' (buf1@out1) op2' (buf2@out2)) \<Longrightarrow>
      le_op op1 buf1 op2 buf2"
 
 primcorec cp where
   "cp = Logic (\<lambda> ev . (cp, [ev])) (LNil)"
-
 
 primcorec lazy_cp where
   "lazy_cp buf = Logic (\<lambda> ev . (lazy_cp (buf@[ev]), [])) (llist_of buf)"
@@ -26,9 +25,8 @@ lemma
 lemma
   "le_op cp (buf'@buf) (lazy_cp buf) buf'"
   apply (coinduction arbitrary: buf buf' rule: le_op.coinduct)
-  apply auto
-  by (metis lappend_llist_of lappend_llist_of_llist_of llist.leq_refl)
-
+  apply simp
+  oops
 
 lemma le_op_trans:
   "le_op op1 buf1 op2 buf2 \<Longrightarrow>
@@ -40,7 +38,7 @@ lemma le_op_trans:
   apply (erule le_op.cases)
   apply (erule le_op.cases)
   apply auto
-  apply (meson surj_pair)
+  apply (meson eq_snd_iff le_op.cases)
   done
 
 primcorec prepend_op where
@@ -56,8 +54,31 @@ lemma prepend_op_Nil[simp]:
     done
   done
 
+lemma lprefix_lshift:
+  "lprefix (xs @@- lxs) (xs @@- lys) \<Longrightarrow>
+   lprefix lxs lys"
+  apply (induct xs arbitrary: lxs lys rule: rev_induct)
+   apply clarsimp+
+  apply (meson LCons_lprefix_LCons)
+  done
 
-lemma
+lemma le_op_same_prefix:      
+  "le_op op1 (xs@ys) op2 (xs@zs) \<Longrightarrow>
+   le_op op1 ys op2 zs"
+  apply (coinduction arbitrary: op1 xs ys zs op2 rule: le_op.coinduct)
+  apply (erule le_op.cases)
+  apply auto
+  using lprefix_lshift apply blast+
+  done
+
+lemma le_op_clean_buffers:      
+  "le_op op1 xs op2 xs \<Longrightarrow>
+   le_op op1 [] op2 []"
+  using le_op_same_prefix
+  by (metis append_Nil2)
+
+
+lemma le_op_antisym:
   "le_op op1 buf1 op2 buf2 \<Longrightarrow>
    le_op op2 buf2 op1 buf1 \<Longrightarrow>
    prepend_op buf1 op1 = prepend_op buf2 op2"
@@ -73,17 +94,114 @@ lemma
     apply (cases "apply op1a x")
     apply (cases "apply op2a x")
     apply auto
-    oops
+    apply (meson le_op.cases prefix_order.dual_order.eq_iff)
+    done
+  subgoal for buf1a op1a buf2a op2a x
+ apply (drule llist.leq_antisym)
+     apply assumption
+    apply auto
+    apply (drule meta_spec[of _ x])+
+    apply (cases "apply op1a x")
+    apply (cases "apply op2a x")
+    apply auto
+    subgoal for op1' out1' op2' out2'    
+      apply (rule exI[of _ op1'])
+      apply (rule exI[of _ "[]"])
+    apply (intro conjI)
+       apply simp
+      apply (rule exI[of _ op2'])
+      apply (rule exI[of _ "[]"])
+      apply simp
+      apply (drule meta_spec)+
+      apply (drule meta_mp)
+      apply (rule refl)
+      apply (drule meta_mp)
+       apply (rule refl)      
+      apply (drule meta_mp)
+       apply (rule refl)      
+      apply (drule meta_mp)
+      apply (rule refl)
+      apply (subgoal_tac "out1' = out2'")
+      subgoal
+        apply hypsubst_thin
+        using le_op_clean_buffers
+        using prefix_order.antisym apply blast
+        done
+      subgoal
+        by (metis le_op.cases prefix_order.antisym_conv same_prefix_prefix)
+      done
+    done
+  subgoal
+    using llist.leq_antisym by blast
+  done
 
-  find_theorems lprefix name: anti
+lemma le_op_refl:
+  "le_op op buf op buf"
+  apply (coinduction arbitrary: op buf  rule: le_op.coinduct)
+  apply auto
+  done
+
+primcorec nil_op where "nil_op = Logic (\<lambda> ev . (nil_op, [])) (LNil)"
+primcorec one_op where "one_op = Logic (\<lambda> ev . (nil_op, [1])) (LNil)"
+primcorec ones_op where "ones_op = Logic (\<lambda> ev . (ones_op, [1])) (LNil)"
+primcorec lazy_ones_op where "lazy_ones_op = Logic (\<lambda> ev . (lazy_ones_op, [])) (repeat 1)"
+primcorec mixed_lazy_ones_op where "mixed_lazy_ones_op = Logic (\<lambda> ev . (lazy_ones_op, [1])) (LNil)"
+
+
+(* primcorec Sup_op :: "('i, 'o) op set \<Rightarrow> ('i, 'o) op"
+where
+  "Sup_op A =
+  (if \<forall>x\<in>A. lnull x then LNil
+   else LCons (THE x. x \<in> lhd ` (A \<inter> {xs. \<not> lnull xs})) (Sup_op (ltl ` (A \<inter> {xs. \<not> lnull xs}))))"
+ *)
+
+definition "(Sup_op:: ('i, 'o) op set \<Rightarrow> ('i, 'o) op) A = undefined"
+
+lemma
+  "Sup_op {} = nil_op"
+  oops
+
+lemma
+  "Sup_op {nil_op, one_op} = one_op"
+  oops
+
+lemma
+  "Sup_op {ones_op, lazy_ones_op} = ones_op"
+  oops
+
+lemma
+  "Sup_op {one_op, lazy_ones_op} = lazy_ones_op"
+  oops
+
+lemma
+  "Sup_op {one_op, ones_op} = ones_op"
+  oops
+
+abbreviation "le_op' buf1 buf2 op1 op2 \<equiv> le_op op1 buf1 op2 buf2"
+
+lemma chain_le_op_Sup_l:
+  "Complete_Partial_Order.chain (le_op' buf1 buf2) A \<Longrightarrow> x \<in> A \<Longrightarrow> (le_op' buf1 buf2) x (Sup_op A)"
+  oops
+
+lemma chain_le_op_Sup_r:
+  "Complete_Partial_Order.chain (le_op' buf1 buf2) A \<Longrightarrow> (\<And>y. y \<in> A \<Longrightarrow> (le_op' buf1 buf2) y x) \<Longrightarrow> (le_op' buf1 buf2) (Sup_op A) x"
+  oops
+
+
+lemma res_ccpo: "class.ccpo Sup_op (le_op' buf1 buf2) (mk_lt res_ord)"
+  apply intro_locales
+(*     apply (rule preorder_mk_ltI)
+      apply unfold_locales
+      apply (auto intro: res_ord_trans res_ord_antisym chain_res_ord_res_Sup_l chain_res_ord_res_Sup_r)
+  done
+   *)
+  oops
 
 primcorec unproduce_op :: "('a llist \<Rightarrow> 'b llist) \<Rightarrow> ('a, 'b) op" where
   "unproduce_op f = 
     (Logic (\<lambda> ev. 
              let out = f (LCons ev LNil) in
-             if lfinite out
-             then (unproduce_op (\<lambda> lxs. ldropn (the_enat (llength out)) (f (LCons ev lxs))), list_of out)
-             else (unproduce_op (\<lambda> _. ltl out), [lhd out]))
+             (unproduce_op (\<lambda> lxs. ldrop (llength out) (f (LCons ev lxs))), list_of out))
            (f LNil))"
 
 
@@ -92,9 +210,31 @@ lemma unproduce_op_correct_1[simp]:
   "produce (unproduce_op f) = f"
   sorry
 
+
 lemma  unproduce_op_correct_2[simp]:
-  "unproduce_op (produce op) = op"
-  sorry
+  "monotone lprefix lprefix (produce op) \<Longrightarrow>
+   unproduce_op (produce op) = op"
+  find_theorems monotone name: "_induc"
+
+
+  oops
+  apply (coinduction arbitrary: op)
+  subgoal for op
+    apply (cases op)
+    apply hypsubst_thin
+    subgoal for lgc exit
+      apply (simp add: rel_fun_def split: list.splits prod.splits if_splits)
+      apply (intro impI conjI allI)
+      subgoal for ev
+      apply (cases "lgc ev")
+        apply simp
+        subgoal for op' out'
+          apply auto
+          subgoal sorry
+          subgoal sorry
+          subgoal
+
+
 
 primcorec incr_Inl where
   "incr_Inl = Logic (\<lambda> ev. 
